This is a work-in-progress commit on SMTLIB generator.
It is intended to provide a checkpoint to the SMTLIB generator before
we try out another approach.

lean/deps/typed_smt2/src/galois/smt2/basic.lean
@@ -2,17 +2,142 @@
 This declares sorts, terms, and semantics for generating SMTLIB
 expressions and reasoning about their interpretation.
 -/
-import galois.data.buffer
-import galois.data.char
-import galois.data.fin
-import galois.data.nat
-import galois.logic
-
 import data.bitvec
-
+import galois.category.except
+import galois.data.buffer
+import galois.data.option
+import galois.logic
 import galois.sexpr
 
 import tactic.find
+
+universes u v
+
+inductive PropExists {α : Prop} (p : α → Prop) : Prop
+| intro (w : α) (h : p w) : PropExists
+
+
+namespace list
+
+def map_with_mem {α} {β: Sort _} : Π(l:list α), (Π(x:α), x ∈ l → β) → list β
+| [] f := []
+| (h::r) f
+  := f h (or.inl rfl)
+  :: map_with_mem r (λ(x:α) (p:x ∈ r), f x (or.inr p))
+
+/- Elements in a list have a smaller size than the list. -/
+theorem mem_sizeof {α} [s : has_sizeof α] {x : α} {l : list α} (p : x ∈ l)
+: sizeof x < l.sizeof :=
+begin
+  induction l,
+  case nil {
+    exact false.elim p,
+  },
+  case cons : h r ind {
+    simp [has_mem.mem, list.mem] at p,
+    simp [list.sizeof, nat.succ_add],
+    apply nat.succ_le_succ,
+    cases p,
+    case or.inl : x_eq_h {
+      simp [x_eq_h],
+    },
+    case or.inr : x_in_r {
+      transitivity, exact le_of_lt (ind x_in_r),
+      apply nat.le_add_right,
+    },
+  },
+end
+
+--- A decidable test for lists using a test for elements that
+-- includes proof only list elements are queried.
+def has_dec_eq_with_mem {α}
+: Π (k l : list α) (p : Π{a : α}, a ∈ k → Π{b:α}, b ∈ l → decidable (a = b)),
+    decidable (k = l)
+| []      [] p    := is_true rfl
+| (a::as) [] p    := is_false (λ h, list.no_confusion h)
+| []      (b::bs) p := is_false (λ h, list.no_confusion h)
+| (a::as) (b::bs) p :=
+  let ma : a ∈ (a::as) := or.inl rfl in
+  let mb : b ∈ (b::bs) := or.inl rfl in
+  match p ma mb with  | is_true hab :=
+    let q (x:α) (xm:x ∈ as) (y:α) (ym:y ∈ bs) :=
+          p (or.inr xm) (or.inr ym) in
+    match has_dec_eq_with_mem as bs q with
+    | is_true habs  :=
+      is_true (eq.subst hab (eq.subst habs rfl))
+    | is_false nabs :=
+      is_false (λ h, list.no_confusion h (λ _ habs, absurd habs nabs))
+    end
+  | is_false nab := is_false (λ h, list.no_confusion h (λ hab _, absurd hab nab))
+  end
+
+/-
+Predicate that returns true if two lists have same length and all
+ pairswise elements are equivalent.
+-/
+inductive holds_pairwise {α} {β} (P : α → β → Prop)
+: list α -> list β -> Prop
+| nil {} : holds_pairwise [] []
+| cons {} {x:α} {xr : list α} {y:β} {yr:list β}
+  : P x y
+  → holds_pairwise xr yr
+  → holds_pairwise (x::xr) (y::yr)
+
+namespace holds_pairwise
+open decidable
+
+/- Decide the holds pairwise relation. -/
+def decide_with_mem {α} {β} (r : α → β → Prop)
+: Π(x:list α) (y:list β),
+   (Π(a:α), a ∈ x → Pi(b:β), b ∈ y → decidable (r a b))
+    → decidable (holds_pairwise r x y)
+| [] [] _ := is_true nil
+| [] (yh::yr) _ := is_false (by { intro p, cases p, })
+| (xh::xr) [] _ := is_false (by { intro p, cases p, })
+| (xh::xr) (yh::yr) p :=
+  match p xh (or.inl rfl) yh (or.inl rfl) with
+  | is_true ph :=
+    let q := λa am b bm, p a (or.inr am) b (or.inr bm) in
+    match decide_with_mem xr yr q with
+    | is_true pr := is_true (cons ph pr)
+    | is_false npr := is_false
+      begin
+        intro p,
+        cases p with x yr y yr ph pr,
+        exact npr pr,
+      end
+    end
+  | is_false nph := is_false
+    begin
+      intro p,
+      cases p with x yr y yr ph pr,
+      exact nph ph,
+    end
+  end
+
+end holds_pairwise
+
+end list
+
+/- A list whose element types are constructed from applying a function to another list. -/
+inductive indexed_list {α:Type u} (f:α → Sort v) : list α → Sort (max (u+1) v)
+| nil {} : indexed_list []
+| cons {h:α} {r:list α} : f h → indexed_list r → indexed_list (h::r)
+
+namespace indexed_list
+section
+
+parameter {α:Type u}
+parameter {f:α → Sort v}
+
+/- Return the nth_le element in the list. -/
+def nth_le : Π{l:list α}, indexed_list f l → Π(i:ℕ) (i_lt:i < l.length), f (l.nth_le i i_lt)
+| ._ nil      n     h := absurd h (nat.not_lt_zero n)
+| ._ (cons a l) 0     h := a
+| ._ (cons a l) (n+1) h := nth_le l n (nat.le_of_succ_le_succ h)
+
+end
+end indexed_list
 
 namespace smt2
 
@@ -93,18 +218,10 @@ def reserved_words : list string :=
 
 def reserved_word := { s:string // s ∈ reserved_words }
 
-instance reserved_word.repr : has_repr reserved_word := ⟨subtype.val⟩
-
-/--
-Construct a reserved word from a character buffer using the decidability of reserved word membership.
--/
-def reserved_word.mk (s:string) (p:as_true (s ∈ reserved_words)) : reserved_word := ⟨s, of_as_true p⟩
-
-
-/-- Reserved words as a list of character buffers. -/
+--- Reserved words as a list of character buffers.
 def reserved_words_buffer : list char_buffer := reserved_words.map string.to_char_buffer
 
-/-- Return true if buffer is a reserved word. -/
+--- Predicate that holds if buffer is a reserved word.
 def is_reserved_word (b:char_buffer) : Prop :=
   b ∈ reserved_words_buffer
 
@@ -112,6 +229,19 @@ namespace is_reserved_word
 local attribute [reducible] is_reserved_word
 instance decidable : decidable_pred is_reserved_word := by apply_instance
 end is_reserved_word
+
+namespace reserved_word
+
+protected def repr : reserved_word → string := subtype.val
+
+instance has_repr : has_repr reserved_word := ⟨reserved_word.repr⟩
+
+/--
+Construct a reserved word from a character buffer using the decidability of reserved word membership.
+-/
+def of_string (s:string) (p:as_true (s ∈ reserved_words)) : reserved_word := ⟨s, of_as_true p⟩
+
+end reserved_word
 
 ------------------------------------------------------------------------
 -- symbol
@@ -151,7 +281,7 @@ end is_symbol
 
 end symbol
 
-/-- This is a simple identifier that can be used in function or symbol names. -/
+/-- A symbol is used to identify function or sort names. -/
 structure symbol :=
 (to_char_buffer : char_buffer)
 (valid : symbol.is_symbol to_char_buffer)
@@ -160,6 +290,7 @@ namespace symbol
 
 instance decidable_eq : decidable_eq symbol := by tactic.mk_dec_eq_instance
 
+--- Reflexive lexicographic ordering of symbols.
 protected def le (x y : symbol) : Prop := x.to_char_buffer ≤ y.to_char_buffer
 instance : has_le symbol := ⟨symbol.le⟩
 instance decidable_le
@@ -170,6 +301,7 @@ begin
   apply_instance,
 end
 
+--- Strict lexicographic ordering of symbols.
 protected def lt (x y : symbol) : Prop := x.to_char_buffer < y.to_char_buffer
 instance : has_lt symbol := ⟨symbol.lt⟩
 instance decidable_lt
@@ -178,6 +310,14 @@ instance decidable_lt
 begin
   simp [has_lt.lt, symbol.lt],
   apply_instance,
+end
+
+/- Sizeof always returns a number greater than 0. -/
+theorem sizeof_gt0 (s:symbol) : symbol.sizeof s > 0 :=
+begin
+  cases s,
+  dsimp [symbol.sizeof],
+  exact dec_trivial,
 end
 
 section simple_symbols
@@ -289,6 +429,51 @@ def is_quoted_symbol (b:char_buffer) : Prop
     else
       is_symbol_char (b.read i)
 
+
+theorem is_quoted_symbol.size_ok {b:char_buffer} : is_quoted_symbol b → 1 ≤ b.size - 1 :=
+begin
+  intro is_sym,
+  apply nat.le_sub_right_of_add_le,
+  dsimp [nat.add_succ],
+  dsimp [is_quoted_symbol] at is_sym,
+  exact is_sym.left,
+end
+
+theorem is_quoted_symbol.symbol_ok {b:char_buffer} (is_sym:is_quoted_symbol b)
+: is_symbol (b.slice 1 (b.size - 1) (is_quoted_symbol.size_ok is_sym)) :=
+begin
+  dsimp [is_symbol],
+  intro i,
+  cases i with i i_lt,
+  simp only [buffer.read_slice],
+
+  --simp [buffer.size_slice] at i_lt,
+
+  have i_p_1 : 1 + i < b.size := buffer.slice_index_bound ⟨i, i_lt⟩,
+
+  -- Introduce forall constraint
+  have q := is_sym.right ⟨1 + i, i_p_1⟩,
+
+  have pr : ¬(1 + i = 0) := by simp,
+
+  have min_le : buffer.size b - 1 ≤ buffer.size b := by apply nat.sub_le_self,
+
+  have sz_pos : b.size > 0 :=
+    calc b.size ≥ 2 : is_sym.left
+            ... > 0 : of_as_true trivial,
+
+  have qr : ¬(1 + i= buffer.size b - 1),
+  { intro q,
+    simp [buffer.size_slice, min_eq_left min_le] at i_lt,
+    simp only [nat.lt_sub_left_iff_add_lt, q] at i_lt,
+    simp [nat.succ_add, nat.sub_succ, nat.succ_pred_eq_of_pos sz_pos, lt_irrefl] at i_lt,
+    exact i_lt,
+  },
+  simp only [fin.val, pr, qr, false_or, if_false] at q,
+  exact q,
+end
+
+
 local attribute [reducible] is_quoted_symbol
 instance is_quoted_symbol.decidable : decidable_pred is_quoted_symbol := by apply_instance
 
@@ -296,42 +481,26 @@ instance is_quoted_symbol.decidable : decidable_pred is_quoted_symbol := by appl
 protected
 def parse (s:string) : except string symbol := do
   let b := s.to_char_buffer,
-  if p:is_simple_symbol b then
+  if pr:is_quoted_symbol b then
+    pure ⟨ b.slice 1 (b.size - 1) (is_quoted_symbol.size_ok pr)
+         , is_quoted_symbol.symbol_ok pr
+         ⟩
+  else if p:is_simple_symbol b then
     pure ⟨b, simple_symbol_is_symbol p⟩
-  else if is_quoted_symbol b then (do
-    let inner : char_buffer := (b.take (b.size - 1)).drop 1,
-    if valid:is_symbol inner then
-      pure ⟨inner, valid⟩
-    else
-      throw "internal symbol parsing inconsistency")
   else
     throw "Invalid symbol"
 
 end parsing
 
+#print tactic.exact_dec_trivial
+-- Construct a reserved word from a character buffer using the decidability of reserved word membership.
+-- def from_decidable (s:char_buffer) (p:as_true (is_symbol s)) : symbol := ⟨s, of_as_true p⟩
 
-/--
-Construct a reserved word from a character buffer using the decidability of reserved word membership.
--/
-def from_decidable (s:char_buffer) (p:as_true (is_symbol s)) : symbol := ⟨s, of_as_true p⟩
+meta def of_string_tac : tactic unit := `[exact trivial]
 
-/-- Map an s-expression to a meta-level expression -/
-protected
-meta def to_expr : symbol → expr
-| ⟨b, p⟩ := do
-  let s : string := b.to_string,
-  let r : reflected _ := `(from_decidable),
-  let f : expr := (`(string.to_char_buffer) : expr).app `(s),
-  ((r : expr).app f).app `(trivial)
+/- Construct a symbol from a string literal. -/
+def of_string (nm:string) (p : (symbol.parse nm).is_ok  . of_string_tac) : symbol := p.value
 
-meta instance : is_meta_string symbol :=
-{ parse := symbol.parse
-, to_expr := symbol.to_expr
-}
-
-/- Construct an atom from a string literal. -/
-def of_string : Π(nm:string), (symbol.parse nm).is_ok → symbol
-| _ p := p.value
 
 theorem is_symbol_append {x y : char_buffer}
 : is_symbol x → is_symbol y → is_symbol (x ++ y) :=
@@ -341,13 +510,11 @@ begin
   intros p q i,
   simp only [buffer.read_append],
   apply (dite (i.val < buffer.size x)),
-  {
-    intro i_lt,
+  { intro i_lt,
     simp [i_lt],
     exact (p _),
   },
-  {
-    intro i_ge,
+  { intro i_ge,
     simp [i_ge],
     exact (q _),
   }
@@ -378,11 +545,8 @@ begin
   exact (nat.nth_to_digits_is_lt (of_as_true trivial) _),
 end
 
-/- Construct an atom from a string literal. -/
+/- Construct a symbol from a string literal. -/
 def of_nat (v : ℕ) : symbol := ⟨string.to_char_buffer (repr v), is_symbol_nat v⟩
-
-def of_prefixed_nat (pre:string) (p : (symbol.parse pre).is_ok) (v : ℕ) : symbol :=
-  of_string pre p ++ of_nat v
 
 end symbol
 
@@ -446,16 +610,6 @@ instance : sexpr.is_atom atom :=
 , read := @atom.read
 }
 
-/-
-protected
-meta def to_expr : atom → expr
-| (symbol s) := `(symbol).to_expr.app s.to_expr
-| (numeral n) := `(numeral).to_expr.app (reflect n).to_expr
-
-
-meta instance has_to_expr_atom : has_to_expr atom := ⟨atom.to_expr⟩
--/
-
 /- Construct an atom from a string literal. -/
 def of_string : Π(nm:string), (char_reader.read_from_string nm (@atom.read _ _ nm.length)).is_ok → atom
 | _ p := p.value
@@ -474,88 +628,703 @@ instance : has_coe symbol (sexpr atom) := ⟨to_sexpr⟩
 end symbol
 
 ------------------------------------------------------------------------
--- identifier
+-- kind
 
-namespace identifier
+/- An parameter for polymorphic declarations. -/
+inductive kind
+| nat  : kind
+| sort : kind
 
-/- An argument to an identifier. -/
-inductive index
-| numeral : ℕ → index
-| symbol : symbol → index
+namespace kind
 
-namespace index
+instance : decidable_eq kind := by tactic.mk_dec_eq_instance
 
-instance : decidable_eq index := by tactic.mk_dec_eq_instance
+/- Map SMTLIB kinds to their Lean interpretation -/
+def interp : kind → Type 1
+| kind.nat := ulift ℕ
+| kind.sort := Type
 
-protected def to_atom : index → atom
-| (numeral n) := atom.numeral n
-| (symbol s)  := atom.symbol s
 
-protected def to_sexpr (i:index) : sexpr atom := sexpr.atom i.to_atom
+end kind
 
-end index
+------------------------------------------------------------------------
+-- sort_arg
 
-instance coe_nat_to_index : has_coe ℕ index := ⟨index.numeral⟩
-instance coe_symbol_to_index : has_coe symbol index := ⟨index.symbol⟩
+/-
+This datatype represents potential arguments to sort paramters, and includes
+parameters, natural number literals, and other sorts.
 
-end identifier
+No requirement is made that the sort is well-formed with respect to a signature.
+-/
+inductive sort_arg (ctx:list kind) : Type
+| nat   {} : ℕ → sort_arg
+| sort  {} : symbol → list sort_arg → sort_arg
+| param {} (i : fin ctx.length) : sort_arg
 
-/- An identifier in SMTLIB possibly with a list of indices as arguments. -/
-structure identifier :=
-(head : symbol)
-(indices : list identifier.index)
 
-namespace identifier
+namespace sort_arg
 
-instance : decidable_eq identifier := by tactic.mk_dec_eq_instance
+------------------------------------------------------------------------
+-- is_child
+
+/- is_child c x holds if one sort_arg appears as an argument to another. -/
+inductive is_child {ctx:list kind} : sort_arg ctx → sort_arg ctx → Prop
+| mem : Π{x : sort_arg ctx} {nm : symbol} {args : list (sort_arg ctx)}
+          (is_mem : x ∈ args),
+          is_child x (sort_arg.sort nm args)
+
+/- Prove is_child relationship is well-founded. -/
+def is_child.wf {ctx:list kind} : well_founded (@is_child ctx) :=
+begin
+  apply well_founded.intro,
+  intro z,
+  apply well_founded.fix (sizeof_measure_wf (sort_arg ctx)) _ z,
+  intros y rec,
+  dsimp [sizeof_measure, measure, inv_image] at rec,
+  apply acc.intro,
+  intros x x_lt_y,
+  cases y with n nm args,
+  { cases x_lt_y, },
+  { cases x_lt_y with a b c x_in_args,
+    apply rec,
+    simp [sizeof, has_sizeof.sizeof, sort_arg.sizeof, nat.succ_add ],
+    transitivity, exact (list.mem_sizeof x_in_args),
+    apply nat.lt_of_le_of_lt (nat.le_add_left _ nm.sizeof),
+    exact (nat.succ_le_succ (nat.le_refl _)),
+  },
+  { cases x_lt_y, },
+end
+
+------------------------------------------------------------------------
+-- fixpoint function based on is_child.
+
+section
+
+parameter {ctx : list kind}
+parameter {C : sort_arg ctx → Sort _}
+parameter (nat_eval : Π(n:ℕ), C (nat n))
+parameter (sort_eval : Π(nm:symbol) (args:list (sort_arg ctx)),
+               (Π(y : sort_arg ctx), y ∈ args → C y)
+               → C (sort nm args))
+parameter (param_eval : Π(i:fin ctx.length), C (param i))
+
+def fix.f
+  : Π (x : sort_arg ctx), (Π (y : sort_arg ctx), sort_arg.is_child y x → C y) -> C x
+| (nat n) _ := nat_eval n
+| (sort nm args) ind := sort_eval nm args (λy h, ind y (is_child.mem h))
+| (param i) _ := param_eval i
+
+@[elab_with_expected_type]
+def fix
+  : Π(x : sort_arg ctx), C x :=
+  well_founded.fix is_child.wf fix.f
+
+end
+
+------------------------------------------------------------------------
+--
+
+/-- Convert a sort_arg to an s-expression. -/
+protected
+def to_sexpr : sort_arg [] → sexpr atom :=
+  let num (n:ℕ) := sexpr.atom (atom.numeral n) in
+  let app (nm : symbol) (args : list (sort_arg [])) rec :=
+        sexpr.parens
+          (sexpr.atom (atom.symbol nm) :: args.map_with_mem rec) in
+  let param_eval (i:fin 0) : sexpr atom := i.elim0 in
+  fix num app param_eval
+
+section decidable
+parameter {ctx : list kind}
+
+def decidable_eq.nat (m:ℕ) : Π(y:sort_arg ctx), decidable (nat m = y)
+| (nat n) :=
+  if p : m = n then
+    is_true (congr_arg nat p)
+  else
+    is_false (λh, p (sort_arg.nat.inj h))
+| (sort nm args) := is_false (by contradiction)
+| (param i)      := is_false (by contradiction)
+
+def decidable_eq.app (nm : symbol) (args : list (sort_arg ctx))
+        (rec : Π(y:sort_arg ctx), y ∈ args → Πz, decidable (y = z))
+ : Π(y:sort_arg ctx), decidable (sort nm args = y)
+ | (nat n) := is_false (by contradiction)
+ | (sort ynm yargs) :=
+   if pnm : nm = ynm then
+     let p (xe) (xmem) (ye) (ymem : ye ∈ yargs)
+          : decidable (xe = ye) := rec xe xmem ye in
+     match list.has_dec_eq_with_mem args yargs p with
+     | is_true pr   := is_true (eq.subst pnm (eq.subst pr rfl))
+     | is_false npr := is_false (λh, npr (sort_arg.sort.inj h).right)
+     end
+   else
+     is_false (λh, pnm (sort_arg.sort.inj h).left)
+| (param i)      := is_false (by contradiction)
+
+def decidable_eq.eval_param (i:fin ctx.length) : Π(y:sort_arg ctx), decidable (param i = y)
+| (nat n) := is_false (by contradiction)
+| (sort nm args) := is_false (by contradiction)
+| (param j)      :=
+  if p : i = j then
+    is_true (congr_arg _ p)
+  else
+    is_false (λh, p (sort_arg.param.inj h))
 
 protected
-def to_sexpr : identifier → sexpr atom
-| ⟨s, []⟩ := s.to_sexpr
-| ⟨s, l⟩  := sexpr.parens (sexpr.of_string "_" trivial :: s :: (index.to_sexpr <$> l))
+def has_dec_eq : decidable_eq (sort_arg ctx) :=
+  fix decidable_eq.nat decidable_eq.app decidable_eq.eval_param
 
-instance : has_coe identifier (sexpr atom) := ⟨identifier.to_sexpr⟩
+instance : decidable_eq (sort_arg ctx) := sort_arg.has_dec_eq
 
-end identifier
+end decidable
+
+end sort_arg
+
+/- Symbol associated with Boolean values. -/
+def symbol.bool : symbol := symbol.of_string "Bool"
+
+------------------------------------------------------------------------
+-- uncurry
+
+/- Map list of kinds for arguments to their interpretation as a function. -/
+def sort_interp (l:list kind) (r:Type 1) : Type 1 := l.foldr (λh r, h.interp → r) r
+
+------------------------------------------------------------------------
+-- sort_model
+
+namespace sort_model
+
+/- Information about a specific sort in the model. -/
+structure info :=
+(params : list kind)
+(interp  : sort_interp params Type)
+
+def bool_info : info := {params := [], interp := Prop}
+
+end sort_model
+
+/-- Defines the mapping from sorts to their parameters and interpretation in Lean. -/
+structure sort_model :=
+(map : rbmap symbol sort_model.info)
+(extends_core : map.find symbol.bool = option.some sort_model.bool_info)
+
+namespace sort_model
+
+/- Defines the core signature, all signatures should extend this. -/
+def core : sort_model :=
+{ map := rbmap.from_list [⟨symbol.bool, sort_model.bool_info⟩]
+, extends_core := rfl
+}
+
+/- Returns the parameters associated with the symbol if any. -/
+def lookup_sort (sig:sort_model) (s:symbol) : option info := sig.map.find s
+
+/- Restate extends_Core in terms of lookup_sort -/
+@[simp]
+theorem lookup_sort_bool (sig:sort_model)
+: lookup_sort sig symbol.bool = option.some sort_model.bool_info := sig.extends_core
+
+
+
+end sort_model
+
+
+------------------------------------------------------------------------
+-- well_formed sort_arg
+
+namespace sort_arg
+
+/- Predicate that indicates if a sort satisfies typing constraints. -/
+inductive well_formed (mdl:sort_model) {ctx : list kind}
+: sort_arg ctx → kind → Prop
+| nat {} (x:ℕ) : well_formed (sort_arg.nat x) kind.nat
+| sort (nm:symbol) (args:list (sort_arg ctx))
+  (p : option.is_some_prop (mdl.lookup_sort nm))
+  : list.holds_pairwise well_formed args p.get.params
+  → well_formed (sort_arg.sort nm args) kind.sort
+| param {} (i:fin ctx.length)
+  : well_formed (param i) (ctx.nth_le i.val i.is_lt)
+
+/- Introduces property implied when we know a sort_arg is a well-defined sort. -/
+theorem well_formed_sort_proof {mdl:sort_model} {ctx : list kind} {nm:symbol} {args:list (sort_arg ctx)}
+(p: well_formed mdl (sort nm args) kind.sort)
+: PropExists
+   (λ(is:option.is_some_prop (mdl.lookup_sort nm)),
+    list.holds_pairwise (well_formed mdl) args is.get.params) :=
+begin
+  cases p with a b c p_p p_a,
+  apply PropExists.intro p_p p_a,
+end
+
+/- Introduces property implied when we know a sort_arg is a well-defined sort. -/
+theorem well_formed.param_proof {mdl:sort_model} {ctx : list kind} {i:fin ctx.length} {k:kind}
+(p: well_formed mdl (param i) k)
+: k = ctx.nth_le i.val i.is_lt :=
+begin
+  cases p,
+  exact rfl,
+end
+
+namespace well_formed
+
+section
+parameter (mdl:sort_model)
+parameter {ctx:list kind}
+
+def decidable.nat (x:ℕ)
+: Π(i:kind), decidable (@well_formed mdl ctx (sort_arg.nat x) i)
+| kind.nat  := is_true (well_formed.nat x)
+| kind.sort := is_false (by {intro p, cases p,})
+
+def decidable.sort
+  (nm:symbol) (args:list (sort_arg ctx))
+  (rec : Π(y), y ∈ args
+    → Π(i:kind), decidable (well_formed mdl y i))
+: Π(i:kind), decidable (well_formed mdl (sort_arg.sort nm args) i)
+| kind.nat  := is_false (by { intro p, cases p, })
+| kind.sort :=
+   if in_f : option.is_some_prop (mdl.lookup_sort nm) then
+     match list.holds_pairwise.decide_with_mem (well_formed mdl) args in_f.get.params
+              (λa am j jm, rec a am j) with
+     | (is_true args_ok) := is_true (well_formed.sort nm args in_f args_ok)
+     | (is_false args_not_ok) :=
+       is_false
+       begin
+         intro p,
+         cases p with a b c psome prest,
+         exact (args_not_ok prest),
+       end
+     end
+   else
+     is_false
+     begin
+       intro p,
+       cases p with a b c psome prest,
+       exact (in_f psome)
+     end
+
+def decidable.eval_param (i:fin ctx.length) (idx:kind)
+: decidable (@well_formed mdl ctx (sort_arg.param i) idx) :=
+  if h : ctx.nth_le i.val i.is_lt = idx then
+    is_true (eq.subst h (well_formed.param i))
+  else
+    is_false begin
+      intro x,
+      cases x,
+      apply h (eq.refl _),
+    end
+
+/-- This returns the type of terms with the given sort. -/
+def decidable
+: Π(s:sort_arg ctx) (i:kind), decidable (well_formed mdl s i) :=
+  @fix ctx
+       (λx, Π(i:kind), decidable (@well_formed mdl ctx x i))
+       decidable.nat
+       decidable.sort
+       decidable.eval_param
+
+end
+end well_formed
+
+------------------------------------------------------------------------
+-- interpretation
+
+
+section term
+
+parameter {mdl:sort_model}
+parameter {ctx : list kind}
+parameter {ctx_args : indexed_list kind.interp ctx}
+
+def type_of.app_args
+        : Π(args : list (sort_arg ctx))
+           (indices : list kind)
+           (i : sort_interp indices Type)
+           (p:list.holds_pairwise (well_formed mdl) args indices)
+           (rec : Π(y), y ∈ args → Π(j:kind), well_formed mdl y j → kind.interp j),
+           Type
+| [] [] d _ rec := d
+| [] (h::r) d p rec := false.elim (by cases p)
+| (h::rest) [] d p rec := false.elim (by cases p)
+| (arg::rest) (idx::r) d p rec := do
+   let is_ok : well_formed mdl arg idx :=
+         begin
+           cases p with a b c d ph pr,
+           exact ph,
+         end in
+   let rest_ok : list.holds_pairwise (well_formed mdl) rest r :=
+         begin
+           cases p with a b c d ph pr,
+           exact pr,
+         end in
+   let v := rec arg (or.inl rfl) idx is_ok in
+   type_of.app_args rest r (d v) rest_ok (λ(y) (p:y ∈ rest), rec y (or.inr p))
+
+def type_of.app (nm:symbol)
+             (args:list (sort_arg ctx))
+             (rec : Π(y), y ∈ args → Π(k:kind), well_formed mdl y k → k.interp)
+: Π(k:kind), well_formed mdl (sort_arg.sort nm args) k → k.interp
+| kind.nat p :=
+  begin
+    apply false.elim,
+    cases p,
+  end
+| kind.sort p :=
+  match well_formed_sort_proof p with
+  | ⟨nm_ok, args_ok⟩ :=
+    let i := nm_ok.get in
+    type_of.app_args args i.params i.interp args_ok rec
+  end
+
+def type_of.num  (n:ℕ)
+: Π(k:kind), well_formed mdl (@sort_arg.nat ctx n) k → k.interp
+| kind.nat _ := ulift.up n
+| kind.sort p :=
+  begin
+    apply false.elim,
+    cases p,
+  end
+
+def type_of.param (i:fin ctx.length)
+: Π(k:kind), well_formed mdl (@sort_arg.param ctx i) k → k.interp
+| k p :=
+  let r := well_formed.param_proof p in
+  cast (congr_arg kind.interp r.symm)
+       (ctx_args.nth_le i.val i.is_lt)
+
+/-- This returns the type of terms with the given sort. -/
+def type_of  : Π(s:sort_arg ctx) (i:kind), well_formed mdl s i → i.interp :=
+  @sort_arg.fix ctx (λs, Π(i), well_formed mdl s i → i.interp) type_of.num type_of.app type_of.param
+
+end term
+
+end sort_arg
 
 ------------------------------------------------------------------------
 -- sort
 
 /-- A type for terms in SMTLIB -/
-def sort : Type := identifier
+inductive sort (mdl:sort_model) (ctx:list kind)
+| named (name  : symbol) (args  : list (sort_arg ctx))
+        (valid : sort_arg.well_formed mdl (sort_arg.sort name args) kind.sort)
+        : sort
+| param {} (i:fin ctx.length) (valid : ctx.nth_le i.val i.is_lt = kind.sort) : sort
 
 namespace sort
-instance : decidable_eq sort := by { unfold sort, apply_instance }
+
+section
+parameter {mdl : sort_model}
+parameter {ctx : list kind}
+
+def to_arg : sort mdl ctx → sort_arg ctx
+| (sort.named nm args _) := sort_arg.sort nm args
+| (sort.param i _)       := sort_arg.param i
+
+instance : has_coe (sort mdl ctx) (sort_arg ctx) := ⟨to_arg⟩
+
+end
 
 protected
-def to_sexpr : sort → sexpr atom := identifier.to_sexpr
+def to_sexpr {mdl : sort_model} (s:sort mdl []) : sexpr atom := s.to_arg.to_sexpr
 
-instance sort_is_sexpr : has_coe sort (sexpr atom) := ⟨sort.to_sexpr⟩
+instance sort_is_sexpr (mdl : sort_model) : has_coe (sort mdl []) (sexpr atom) := ⟨sort.to_sexpr⟩
+
+section
+parameter {mdl : sort_model}
+parameter {ctx : list kind}
+
+protected
+def has_dec_eq : decidable_eq (sort mdl ctx)
+| (sort.named xnm xargs _) (sort.named ynm yargs _) :=
+  if ph : xnm = ynm then
+    if pr : xargs = yargs then
+      is_true (by simp [ph, pr])
+    else
+      is_false (λh, pr (sort.named.inj h).right)
+  else
+    is_false (λh, ph (sort.named.inj h).left)
+| (sort.named _ _ _) (sort.param _ _) := is_false (λh, sort.no_confusion h)
+| (sort.param _ _) (sort.named _ _ _) := is_false (λh, sort.no_confusion h)
+| (sort.param i _) (sort.param j _) :=
+  if ph:i = j then
+    is_true (by simp [ph])
+  else
+    is_false (λh, ph (sort.param.inj h))
+
+instance : decidable_eq (sort mdl ctx) := sort.has_dec_eq
+
+end
+
+/- Attempt to construct a parameter using decidabile relations. -/
+def by_param {mdl:sort_model}
+                   (ctx:list kind)
+                   (i:ℕ)
+                   (p : as_true (i < ctx.length) . symbol.of_string_tac)
+                   (q : as_true (ctx.nth_le i (of_as_true p) = kind.sort) . symbol.of_string_tac)
+: sort mdl ctx := sort.param ⟨i, of_as_true p⟩ (of_as_true q)
 
 end sort
 
-/-- Denotes Booleans -/
-def bool : sort := ⟨symbol.of_string "bool" trivial, []⟩
+/-- Sort associated with Boolean values. -/
+def sort.bool {mdl:sort_model} {ctx:list kind} : sort mdl ctx :=
+  sort.named symbol.bool []
+    (@sort_arg.well_formed.sort mdl ctx symbol.bool []
+       (begin simp [sort_model.lookup_sort_bool], exact dec_trivial, end)
+       (begin simp [sort_model.lookup_sort_bool], apply list.holds_pairwise.nil, end))
 
 ------------------------------------------------------------------------
--- inhabited_type
+-- signature
 
-/-- A type with a default value in that type. -/
-structure inhabited_type :=
-(type : Type)
-(value : type)
+inductive fun_attr
+| left_assoc : fun_attr
+| right_assoc : fun_attr
+| chainable : fun_attr
+| pairwise : fun_attr
 
-namespace inhabited_type
+structure fun_signature (sig:sort_model) : Type 1 :=
+(params : list kind := [])
+(args   : list (sort sig params) := [])
+(return : sort sig params)
+(attrs : option fun_attr := none)
 
-def bool : inhabited_type := { type := Prop, value := true }
+/- A function declaration. -/
+def fun_decl (sig:sort_model) := symbol × fun_signature sig
 
-/-- A type with natural numbers that can be used for uninterpreted values. -/
-def uninterpreted : inhabited_type := { type := ℕ, value := 0 }
+def declare_fun {sig:sort_model} (nm:string)
+   (params : list kind)
+   (args   : list (sort sig params))
+   (ret:sort sig params)
+   (attrs : option fun_attr := none)
+   (p : (symbol.parse nm).is_ok  . symbol.of_string_tac)
+   : fun_decl sig :=
+  (symbol.of_string nm p, { params := params, args := args, return := ret, attrs := attrs })
 
-end inhabited_type
+def declare_bin {sig:sort_model} (nm:string)
+   (params : list kind)
+   (s     : sort sig params)
+   (attrs : option fun_attr := none)
+   (p : (symbol.parse nm).is_ok  . symbol.of_string_tac)
+   : fun_decl sig :=
+  declare_fun nm params [s,s] s attrs p
 
-------------------------------------------------------------------------
--- logic
+inductive sort_args : list kind → Type 1
+| nil : sort_args []
+| cons {h:kind} {r:list kind} (x:h.interp) (l:sort_args r) : sort_args (h::r)
+
+def provide : Π(ctx:list kind), (sort_args ctx → Type 1) → Type 1
+| [] f := f sort_args.nil
+| (h::r) f := Π(x:h.interp), provide r (λargs, f (sort_args.cons x args))
+
+def sort_arg.interp {sig:sort_model}
+: Π{ctx:list kind} (s:sort_arg ctx) (k:kind), sort_arg.well_formed sig s k → sort_args ctx → Type 1
+| ._ (sort_arg.sort _ _) _ _ sort_args.nil := sorry
+| ._ s (sort_args.cons h r) := sorry
+
+
+def declare_rel {sig:sort_model} (nm:string)
+   (params : list kind)
+   (s     : sort sig params)
+   (d     : provide params (λargs, s.interp args → s.interp args → Prop))
+   (attrs : option fun_attr := none)
+   (p : (symbol.parse nm).is_ok  . symbol.of_string_tac)
+   : fun_decl sig :=
+  declare_fun nm params [s,s] sort.bool attrs p
+
+
+open fun_attr
+
+/-- The core function declarations. -/
+def core_fun_decls (sig:sort_model) : list (fun_decl sig) :=
+  let ctx := [kind.sort] in
+  let param0 : sort sig ctx := sort.by_param ctx 0 in
+  [ declare_fun "true"  [] []  sort.bool
+  , declare_fun "false" [] []  sort.bool
+  , declare_fun "not"   [] [sort.bool]  sort.bool
+  , declare_bin "=>"    [] sort.bool right_assoc
+  , declare_bin "and"   [] sort.bool left_assoc
+  , declare_bin "or"    [] sort.bool left_assoc
+  , declare_bin "xor"   [] sort.bool left_assoc
+  , declare_rel "="        ctx param0 chainable
+  , declare_rel "distinct" ctx param0 pairwise
+  , declare_fun "ite"      ctx [sort.bool, param0, param0] param0
+  ]
+
+/-- This is a signature for sorts and functions. -/
+structure signature :=
+(sorts : sort_model)
+(functions : rbmap symbol (fun_signature sorts))
+
+namespace signature
+
+def from_fun_decls (sig:sort_model)
+
+
+def core : signature := sorry
+
+/-
+def fun_signature (sig:signature) :
+
+/-- Return the indices associated with the given symbol. -/
+def sort_interp (m:sort_interp_map) (nm:symbol) : option sort_interp := m.map.find nm
+
+/-- Return the indices associated with the given symbol. -/
+def symbol_indices (m:sort_interp_map) (nm:symbol) : option (list kind) :=
+  option.map sort_interp.indices (m.sort_interp nm)
+
+/-- Holds when the sort arg is well formed with the given kind type. -/
+def sort_arg_ok (m:sort_interp_map) : sort_arg → kind → Prop :=
+  sort_arg.well_defined (symbol_indices m)
+-/
+
+end signature
+
+
+namespace sort_arg
+
+/-
+section term
+
+parameter (m:sort_interp_map)
+
+def term.app_args
+        : Π(args:list sort_arg)
+           (i:sort_interp)
+           (p:holds_pairwise m.sort_arg_ok
+                             args
+                             i.indices)
+           (rec : Π(y), y ∈ args → Π(j:kind), m.sort_arg_ok y j → kind.domain j),
+           Type
+| [] ⟨[],d⟩ _ rec := d
+| [] ⟨h::r,d⟩ p rec := false.elim (by cases p)
+| (h::rest) ⟨[],d⟩ p rec := false.elim (by cases p)
+| (arg::rest) ⟨idx::r,d⟩ p rec := do
+   let is_ok : m.sort_arg_ok arg idx :=
+         begin
+           cases p with a b c d ph pr,
+           exact ph,
+         end in
+   let rest_ok : holds_pairwise m.sort_arg_ok  rest r :=
+         begin
+           cases p with a b c d ph pr,
+           exact pr,
+         end in
+   let v := rec arg (or.inl rfl) idx is_ok in
+   term.app_args rest ⟨r,d v⟩ rest_ok (λ(y) (p:y ∈ rest), rec y (or.inr p))
+
+theorem well_defined_sort_proof {nm:symbol} {args:list sort_arg}
+(p: sort_arg.well_defined m.symbol_indices (sort_arg.sort_app nm args) kind.sort)
+: PropExists
+   (λ(is:option.is_some_prop (m.symbol_indices nm)),
+    holds_pairwise (sort_arg.well_defined m.symbol_indices) args is.get) :=
+begin
+  cases p with a b c p_p p_a,
+  apply PropExists.intro p_p p_a,
+end
+
+def term.app (nm:symbol) (args:list sort_arg)
+             (rec : Π(y), y ∈ args → Π(i:kind), m.sort_arg_ok y i → kind.domain i)
+: Π(i:kind), m.sort_arg_ok (sort_arg.sort_app nm args) i → kind.domain i
+| kind.numeral p :=
+  begin
+    apply false.elim,
+    simp [sort_interp_map.sort_arg_ok] at p,
+    cases p,
+  end
+| kind.sort p :=
+  match well_defined_sort_proof p with
+  | ⟨nm_ok, args_ok⟩ :=
+    let interp : sort_interp := ((option.is_some_prop_map (m.sort_interp nm) sort_interp.indices).mp nm_ok).get in
+    let args_ok' : holds_pairwise (sort_arg.well_defined m.symbol_indices) args interp.indices :=
+          begin
+            simp [ option.get_is_some_prop_map (m.sort_interp nm) sort_interp.indices],
+            exact args_ok,
+          end in
+    term.app_args args interp args_ok' rec
+  end
+
+def term.num (x:ℕ)
+: Π(i:kind), m.sort_arg_ok (sort_arg.numeral x) i → kind.domain i
+| kind.numeral _ := ulift.up x
+| kind.sort p :=
+  begin
+    apply false.elim,
+    simp [sort_interp_map.sort_arg_ok] at p,
+    cases p,
+  end
+
+
+/-- This returns the type of terms with the given sort. -/
+def term : Π(s:sort_arg) (i:kind), m.sort_arg_ok s i → i.domain :=
+  @sort_arg.fix (λs, Π(i), m.sort_arg_ok s i → i.domain) term.num term.app
+
+end term
+-/
+
+end sort_arg
+
+namespace term
+
+section
+
+parameter (m:sort_interp_map)
+
+def well_formed (s:sort) : Prop := sort_arg.well_defined m.symbol_indices s kind.sort
+
+def term (s:sort) (p:well_formed s) : Type := sort_arg.term m (s.to_arg) kind.sort p
+
+end
+
+end term
+
+/-
+section get_term
+
+parameter (m:rbmap symbol sort_interp)
+
+def get_term.app_args (nm:symbol)
+        : sort_interp
+        → Π(args:list sort_arg) (rec : Π(y), y ∈ args → except string Type),
+           except string Type
+| ⟨[],d⟩ [] rec := except.ok (d : Type)
+| ⟨h::r,d⟩ [] rec := except.error ("Not enough arguments to " ++ repr nm)
+| ⟨[],d⟩ (h::rest) rec := except.error ("Too many arguments to " ++ repr nm)
+| ⟨kind.numeral::r,d⟩ (arg :: rest) rec := do
+   match arg with
+   | (numeral n) :=
+     get_term.app_args ⟨r,d ⟨n⟩⟩ rest (λ(y) (p:y ∈ rest), rec y (or.inr p))
+   | (sort_app nm args) :=
+      except.error "Cannot supply sort to numeric sort parameter."
+   end
+| ⟨kind.sort::r,d⟩ (arg::rest) rec := do
+   v ← rec arg (or.inl rfl),
+   get_term.app_args ⟨r,d v⟩ rest (λ(y) (p:y ∈ rest), rec y (or.inr p))
+
+def get_term.app (nm:symbol) (args:list sort_arg)
+                (rec : Π(y), y ∈ args → except string Type)
+: except string Type :=
+  match rbmap.find m nm with
+  | option.none := except.error ("Undefined sort " ++ repr nm)
+  | (option.some d) := get_term.app_args nm d args rec
+  end
+
+def get_term.num (x:ℕ) : except string Type :=
+  except.error "Cannot get type of numeric argument."
+
+/-- This returns the type of terms with the given sort. -/
+def get_term (s:sort_arg) : except string Type :=
+  @fix (λx, except string Type) get_term.num (get_term.app m) s
+
+end get_term
+-/
+
+inductive bool_term (m:sort_interp_map) (f : Π(s:sort), sort.well_formed m s → Type) : Type
+| eq (s:sort) (x y : f s) : bool_term
+
+
+def sort_interp.bool (f : sort → Type) : sort_interp :=
+{ indices := [], term := bool_term f }
+
 
 /--
 This defines an interpretation of sorts.
@@ -566,54 +1335,58 @@ be Prop.
 As there are an unbounded number of sorts, implementations should map
 the ones they recognize to the appropriate type, then map the others
 to `inhabited_type.uninterpreted` to represent uninterpreted types.
-
-We use a function rather than finite map to deal with polymorphic
-types such as bitvectors.
 -/
 structure logic :=
-(interpretation : sort → inhabited_type)
-(bool_correct : (interpretation bool).type = Prop)
+(sort_map : rbmap symbol sort_interp)
+(bool_correct :  sort_arg.term bool.to_arg sort_map = bool_term )
+
+namespace sort
+
+/-- This returns the type of sort arguments (and errors for numeric ones) -/
+def get_type_of (s:sort) (l:logic) : except string Type :=
+  s.to_arg.type_of l.sort_map
+
+-- This returns the type of sort arguments (and errors for numeric ones)
+def type_of (s:sort) (l:logic) (p:(get_type_of s l).is_ok) : Type := p.value
+
+end sort
+
 
 namespace logic
 
---- Return the type associated with the given sort or Prop if not defined
-def type_of (l:logic) (s:sort) : Type := (l.interpretation s).type
+-- Coercision from prop to l.type_of bool
+--def of_prop (l:logic) (x:Prop) : bool.type_of l := cast (eq.symm l.bool_correct) x
 
--- Assert proposition is assigned to Booleans
---def prop_is_bool_type (l:logic) : l.type_of bool = inhabited_type.bool := l.bool_correct
+-- Coercision from prop to l.type_of bool
+--def to_prop (l:logic) (x:l.type_of bool) : Prop := cast l.bool_correct x
 
-/-- Coercision from prop to l.type_of bool -/
-def of_prop (l:logic) (x:Prop) : l.type_of bool := cast (eq.symm l.bool_correct) x
+-- @fun_type args res@ dReturn the type assigned to functions. -/
+--def fun_domain (l:logic) : list sort → sort → Type
+--| [] res := l.type_of res
+--| (h::r) s := l.type_of h → fun_domain r s
 
-/-- Coercision from prop to l.type_of bool -/
-def to_prop (l:logic) (x:l.type_of bool) : Prop := cast l.bool_correct x
+-- Return the type associated with the given sort or Prop if not defined
+--def value_of (l:logic) (s:sort) : l.type_of s := (l.interpretation s).value
 
-/-- @fun_type args res@ dReturn the type assigned to functions. -/
-def fun_domain (l:logic) : list sort → sort → Type
-| [] res := l.type_of res
-| (h::r) s := l.type_of h → fun_domain r s
-
---- Return the type associated with the given sort or Prop if not defined
-def value_of (l:logic) (s:sort) : l.type_of s := (l.interpretation s).value
-
---- Default value for a function
-def fun_default_value (l:logic) : Π(args:list sort) (res:sort), l.fun_domain args res
-| [] res := l.value_of res
-| (h::r) tp := λ(x : l.type_of h), fun_default_value r tp
+-- Default value for a function
+--def fun_default_value (l:logic) : Π(args:list sort) (res:sort), l.fun_domain args res
+--| [] res := l.value_of res
+--| (h::r) tp := λ(x : l.type_of h), fun_default_value r tp
 
 end logic
 
 ------------------------------------------------------------------------
 -- Model
 
-/--
-Provides a valuation of symbols in a SMT formula.  This is parameterized by a logic, which
-defines how SMTLIB sorts should be mapped to Lean types.
+/-- Provides a valuation of symbols in a SMT formula.  This is
+parameterized by a logic, which defines how SMTLIB sorts should be
+mapped to Lean types.
 
-This maps symbols (which could be functions) to their type information and a valuation with
-the write domain according to the logic.
--/
-def model (l:logic) : Type := rbmap symbol (Σ(args:list sort) (s:sort), l.fun_domain args s)
+This maps symbols (which could be functions) to their type information
+and a valuation with the correct domain according to the logic.  -/
+
+def model (l:logic) : Type := rbmap symbol (Σ(args:list sort) (s:sort),
+l.fun_domain args s)
 
 instance (l:logic) : has_emptyc (model l) :=
 { emptyc := mk_rbmap _ _ }
@@ -766,3 +1539,20 @@ def is_string_lit (b:char_buffer) : Prop :=
   ∀(i:fin b.size), is_string_lit_char (b.read i)
 
 end smt2
+
+------------------------------------------------------------------------
+-- inhabited_type
+
+/-- A type with a default value in that type. -/
+structure inhabited_type :=
+(type : Type)
+(value : type)
+
+namespace inhabited_type
+
+def bool : inhabited_type := { type := Prop, value := true }
+
+/-- A type with natural numbers that can be used for uninterpreted values. -/
+def uninterpreted : inhabited_type := { type := ℕ, value := 0 }
+
+end inhabited_type
